Definition and proof for fully instantiated version of AES-256

silveroak-opentitan/aes/Spec/Tests/CipherTest.v
@@ -24,6 +24,7 @@ Require Import AesSpec.Placeholder.MixColumns.
 Require Import AesSpec.AddRoundKey.
 Require Import AesSpec.ShiftRows.
 Require Import AesSpec.SubBytes.
+Require Import AesSpec.StateTypeConversions.
 Local Open Scope string_scope.
 
 Local Notation byte := Byte.byte (only parsing).
@@ -32,57 +33,6 @@ Local Notation state := (Vector.t bool 128) (only parsing).
 Local Notation bytes_per_word := 4%nat.
 Local Notation bits_per_word := (bytes_per_word * 8)%nat.
 Local Notation Nb := 4%nat.
-
-(* Conversions between different representations of the state *)
-Section Conversions.
-  (* Notes on representation:
-
-     Everything in FIPS is big-endian, while Coq's native bitvectors are
-     little-endian. The flat bit-vector for the state is therefore
-     little-endian, while rows/columns created from it use the big-endian
-     representation.
-
-     For interpretation as a 2-D matrix, bytes in the flat representation are in
-     *column-major* order (see FIPS 197 Fig. 3) *)
-
-  Definition to_big_endian_bytes (st : state) : Vector.t byte (bytes_per_word * Nb) :=
-    (* byte conversion expects little-endian form *)
-    let bytes := bitvec_to_bytevec (bytes_per_word * Nb) st in
-    (* reverse to get big-endian *)
-    reverse bytes.
-  Definition from_big_endian_bytes (bytes : Vector.t byte (bytes_per_word * Nb)) : state :=
-    let bytes := reverse bytes in (* change to little-endian *)
-    (* byte conversion expects little-endian form *)
-    bytevec_to_bitvec _ bytes.
-
-  (* Convert 1-D state to/from 2-D arrays *)
-  Definition to_cols (st : state) : Vector.t (Vector.t byte bytes_per_word) Nb :=
-    reshape (to_big_endian_bytes st).
-  Definition to_rows (st : state) : Vector.t (Vector.t byte Nb) bytes_per_word :=
-    transpose (to_cols st).
-  Definition from_rows (v : Vector.t (Vector.t byte Nb) bytes_per_word) : state :=
-    from_big_endian_bytes (flatten (transpose v)).
-  Definition from_cols (v : Vector.t (Vector.t byte bytes_per_word) Nb) : state :=
-    from_big_endian_bytes (flatten v).
-
-  (* Convert state to/from columns, but such that columns are bits (still
-     big-endian) instead of bytes *)
-  Definition to_cols_bits (st : state) : Vector.t (Vector.t bool bits_per_word) Nb :=
-    let cols := to_cols st in
-    (* byte conversion expects little-endian form, so reverse each column and
-       then reverse back *)
-    map (fun c => reverse (bytevec_to_bitvec _ (reverse c))) cols.
-  Definition from_cols_bits (bits : Vector.t (Vector.t bool bits_per_word) Nb)
-    : state := from_cols (map (fun c => reverse (bitvec_to_bytevec _ (reverse c))) bits).
-
-  (* Convert state to/from rows, but as lists instead of vectors *)
-  Definition to_list_rows (st : state) : list (list Byte.byte) :=
-    to_list (map to_list (to_rows st)).
-  Definition from_list_rows (rows : list (list Byte.byte)) : state :=
-    let rows := List.map (of_list_sized Byte.x00 bytes_per_word) rows in
-    let rows := of_list_sized (Vector.const Byte.x00 _) Nb rows in
-    from_rows rows.
-End Conversions.
 
 Definition add_round_key (k : round_key) (st : state) : state :=
   let st := to_cols_bits st in
