silveroak-opentitan/aes/Acorn/AddRoundKey.v
@@ -22,6 +22,7 @@ Require Import Cava.VectorUtils.
 Require Import Cava.Acorn.Acorn.
 Require Import Cava.Lib.BitVectorOps.
 Require Import AcornAes.Common.
+Require Import AesSpec.StateTypeConversions.
 Require Import AesSpec.Tests.CipherTest.
 Require Import AesSpec.Tests.Common.
 Import Common.Notations.
