silveroak-opentitan/aes/Spec/FullCipher.v
@@ -1,0 +1,120 @@
+(****************************************************************************)
+(* Copyright 2020 The Project Oak Authors                                   *)
+(*                                                                          *)
+(* Licensed under the Apache License, Version 2.0 (the "License")           *)
+(* you may not use this file except in compliance with the License.         *)
+(* You may obtain a copy of the License at                                  *)
+(*                                                                          *)
+(*     http://www.apache.org/licenses/LICENSE-2.0                           *)
+(*                                                                          *)
+(* Unless required by applicable law or agreed to in writing, software      *)
+(* distributed under the License is distributed on an "AS IS" BASIS,        *)
+(* WITHOUT WARRANTIES OR CONDITIONS OF ANY KIND, either express or implied. *)
+(* See the License for the specific language governing permissions and      *)
+(* limitations under the License.                                           *)
+(****************************************************************************)
+
+(* This file has the top-level cipher definition and proofs, with all the
+   subroutines instantiated. *)
+
+Require Import Coq.Lists.List.
+Require Import Cava.ListUtils.
+Require Import AesSpec.AddRoundKey.
+Require Import AesSpec.Placeholder.MixColumns.
+Require Import AesSpec.ShiftRows.
+Require Import AesSpec.SubBytes.
+Require Import AesSpec.Cipher.
+Require Import AesSpec.CommuteProperties.
+Require Import AesSpec.StateTypeConversions.
+
+(* TODO: these definitions need to be filled in once the mixcolumns spec is finalized *)
+Axiom inverse_mix_columns :
+  forall Nb (st : Vector.t _ Nb), inv_mix_columns (mix_columns st) = st.
+
+(*
+Axiom mix_columns_add_round_key_comm :
+  forall st k,
+    add_round_key
+      32 4
+      (to_cols_bits (from_cols (inv_mix_columns (to_cols (from_cols_bits st)))))
+      (to_cols_bits (from_cols (inv_mix_columns (to_cols (from_cols_bits k)))))
+    = to_cols_bits
+        (from_cols
+           (inv_mix_columns
+              (to_cols (from_cols_bits
+                          (add_round_key 32 4 st k))))).
+*)
+Axiom mix_columns_add_round_key_comm :
+  forall (st k : Vector.t _ 4),
+    let to_bits x := to_cols_bits (from_cols x) in
+    let from_bits x := to_cols (from_cols_bits x) in
+    add_round_key 32 4
+                  (to_bits (inv_mix_columns st))
+                  (to_bits (inv_mix_columns k))
+    = to_bits
+        (inv_mix_columns
+           (from_bits
+              (add_round_key
+                 32 4 (to_bits st) (to_bits k)))).
+
+Section Equivalence.
+  Let state := Vector.t bool 128.
+  Let round_key := Vector.t bool 128.
+  Let bits_per_word := 32.
+  Let Nb := 4%nat. (* From FIPS -- number of bytes per word *)
+  Let Nr := 14%nat. (* From FIPS -- number of rounds *)
+
+  Definition add_round_key (st : state) (k : round_key) : state :=
+    let st := to_cols_bits st in
+    let k := to_cols_bits k in
+    from_cols_bits (add_round_key bits_per_word Nb st k).
+
+  Definition sub_bytes (st : state) : state :=
+    from_list_rows (sub_bytes (to_list_rows st)).
+
+  Definition shift_rows (st : state) : state :=
+    from_list_rows (shift_rows (to_list_rows st)).
+
+  Definition mix_columns (st : state) : state :=
+    from_cols (mix_columns (to_cols st)).
+
+  Definition inv_sub_bytes (st : state) : state :=
+    from_list_rows (inv_sub_bytes (to_list_rows st)).
+
+  Definition inv_shift_rows (st : state) : state :=
+    from_list_rows (inv_shift_rows (to_list_rows st)).
+
+  Definition inv_mix_columns (st : state) : state :=
+    from_cols (inv_mix_columns (to_cols st)).
+
+  Definition aes256_encrypt
+             (first_key last_key : round_key) (middle_keys : list round_key)
+             (input : state) : state :=
+    cipher state round_key add_round_key sub_bytes shift_rows mix_columns
+           first_key last_key middle_keys input.
+
+  Definition aes256_decrypt
+             (first_key last_key : round_key) (middle_keys : list round_key)
+             (input : state) : state :=
+    equivalent_inverse_cipher
+      state round_key add_round_key inv_sub_bytes inv_shift_rows inv_mix_columns
+      last_key first_key (map inv_mix_columns (rev middle_keys)) input.
+
+  Hint Rewrite @inverse_add_round_key @inverse_shift_rows @inverse_sub_bytes
+       @inverse_mix_columns @sub_bytes_shift_rows_comm @mix_columns_add_round_key_comm
+       using solve [eauto] : inverse.
+
+  Lemma aes256_decrypt_encrypt first_key last_key middle_keys input :
+    aes256_decrypt first_key last_key middle_keys
+                   (aes256_encrypt first_key last_key middle_keys input) = input.
+  Proof.
+    cbv [aes256_decrypt aes256_encrypt].
+    eapply inverse_cipher_id; intros.
+    all:cbv [add_round_key sub_bytes shift_rows mix_columns
+                           inv_sub_bytes inv_shift_rows inv_mix_columns].
+    all:autorewrite with conversions inverse.
+    all:reflexivity.
+  Qed.
+End Equivalence.
+
+Redirect "FullCipherAssumptions" Print Assumptions aes256_decrypt_encrypt.
