silveroak-opentitan/aes/Spec/StateTypeConversions.v
@@ -1,0 +1,190 @@
+(****************************************************************************)
+(* Copyright 2020 The Project Oak Authors                                   *)
+(*                                                                          *)
+(* Licensed under the Apache License, Version 2.0 (the "License")           *)
+(* you may not use this file except in compliance with the License.         *)
+(* You may obtain a copy of the License at                                  *)
+(*                                                                          *)
+(*     http://www.apache.org/licenses/LICENSE-2.0                           *)
+(*                                                                          *)
+(* Unless required by applicable law or agreed to in writing, software      *)
+(* distributed under the License is distributed on an "AS IS" BASIS,        *)
+(* WITHOUT WARRANTIES OR CONDITIONS OF ANY KIND, either express or implied. *)
+(* See the License for the specific language governing permissions and      *)
+(* limitations under the License.                                           *)
+(****************************************************************************)
+
+Require Import Coq.Vectors.Vector.
+Require Import Cava.BitArithmetic.
+Require Import Cava.ListUtils.
+Require Import Cava.VectorUtils.
+
+Local Notation byte := Byte.byte (only parsing).
+Local Notation state := (Vector.t bool 128) (only parsing).
+Local Notation bytes_per_word := 4%nat.
+Local Notation bits_per_word := (bytes_per_word * 8)%nat.
+Local Notation Nb := 4%nat.
+
+(* Conversions between different representations of the state *)
+Section Conversions.
+  (* Notes on representation:
+
+     Everything in FIPS is big-endian, while Coq's native bitvectors are
+     little-endian. The flat bit-vector for the state is therefore
+     little-endian, while rows/columns created from it use the big-endian
+     representation.
+
+     For interpretation as a 2-D matrix, bytes in the flat representation are in
+     *column-major* order (see FIPS 197 Fig. 3) *)
+
+  Definition to_big_endian_bytes (st : state) : Vector.t byte (bytes_per_word * Nb) :=
+    (* byte conversion expects little-endian form *)
+    let bytes := bitvec_to_bytevec (bytes_per_word * Nb) st in
+    (* reverse to get big-endian *)
+    reverse bytes.
+  Definition from_big_endian_bytes (bytes : Vector.t byte (bytes_per_word * Nb)) : state :=
+    let bytes := reverse bytes in (* change to little-endian *)
+    (* byte conversion expects little-endian form *)
+    bytevec_to_bitvec _ bytes.
+
+  (* Convert 1-D state to/from 2-D arrays *)
+  Definition to_cols (st : state) : Vector.t (Vector.t byte bytes_per_word) Nb :=
+    reshape (to_big_endian_bytes st).
+  Definition to_rows (st : state) : Vector.t (Vector.t byte Nb) bytes_per_word :=
+    transpose (to_cols st).
+  Definition from_cols (v : Vector.t (Vector.t byte bytes_per_word) Nb) : state :=
+    from_big_endian_bytes (flatten v).
+  Definition from_rows (v : Vector.t (Vector.t byte Nb) bytes_per_word) : state :=
+    from_cols (transpose v).
+
+  (* Convert state to/from columns, but such that columns are bits (still
+     big-endian) instead of bytes *)
+  Definition to_cols_bits (st : state) : Vector.t (Vector.t bool bits_per_word) Nb :=
+    let cols := to_cols st in
+    (* byte conversion expects little-endian form, so reverse each column and
+       then reverse back *)
+    map (fun c => reverse (bytevec_to_bitvec _ (reverse c))) cols.
+  Definition from_cols_bits (bits : Vector.t (Vector.t bool bits_per_word) Nb)
+    : state := from_cols (map (fun c => reverse (bitvec_to_bytevec _ (reverse c))) bits).
+
+  (* Convert state to/from rows, but as lists instead of vectors *)
+  Definition to_list_rows (st : state) : list (list Byte.byte) :=
+    to_list (map to_list (to_rows st)).
+  Definition from_list_rows (rows : list (list Byte.byte)) : state :=
+    let rows := of_list_sized (@List.nil _) Nb rows in
+    let rows := map (of_list_sized Byte.x00 bytes_per_word) rows in
+    from_rows rows.
+End Conversions.
+
+Section Properties.
+
+  Hint Rewrite @bytevec_to_bitvec_to_bytevec @bitvec_to_bytevec_to_bitvec
+       @reverse_reverse @reshape_flatten @flatten_reshape @transpose_involutive
+       @of_list_sized_to_list
+  : inverse.
+
+  Local Ltac inverse :=
+    repeat first [ progress autorewrite with inverse
+                 | rewrite map_map
+                 | apply map_id_ext; intros
+                 | rewrite map_id_ext by (intros; inverse)
+                 | reflexivity ].
+
+  Lemma to_big_endian_bytes_from_big_endian_bytes bytes :
+    to_big_endian_bytes (from_big_endian_bytes bytes) = bytes.
+  Proof.
+    cbv [to_big_endian_bytes from_big_endian_bytes].
+    inverse.
+  Qed.
+  Hint Rewrite to_big_endian_bytes_from_big_endian_bytes : inverse.
+
+  Lemma to_cols_from_cols cols :
+    to_cols (from_cols cols) = cols.
+  Proof. cbv [to_cols from_cols]. inverse. Qed.
+  Hint Rewrite to_cols_from_cols : inverse.
+
+  Lemma to_cols_bits_from_cols_bits bits :
+    to_cols_bits (from_cols_bits bits) = bits.
+  Proof. cbv [to_cols_bits from_cols_bits]. inverse. Qed.
+  Hint Rewrite to_cols_bits_from_cols_bits : inverse.
+
+  Lemma to_rows_from_rows rows :
+    to_rows (from_rows rows) = rows.
+  Proof. cbv [to_rows from_rows]. inverse. Qed.
+  Hint Rewrite to_rows_from_rows : inverse.
+
+  Lemma to_list_rows_from_list_rows rows :
+    length rows = bytes_per_word ->
+    (forall r, List.In r rows -> length r = Nb) ->
+    to_list_rows (from_list_rows rows) = rows.
+  Proof.
+    intros Hlen_rows Hlen_r.
+    cbv [to_list_rows from_list_rows]; intros.
+    inverse. cbv [of_list_sized].
+    autorewrite with push_to_list.
+    erewrite List.map_ext_in
+      by (intros; autorewrite with push_to_list;
+          reflexivity).
+    apply ListUtils.map_id_ext; reflexivity.
+  Qed.
+  Hint Rewrite to_list_rows_from_list_rows : inverse.
+
+  Lemma to_list_rows_length_outer st :
+    length (to_list_rows st) = bytes_per_word.
+  Proof.
+    cbv [to_list_rows].
+    autorewrite with push_length.
+    reflexivity.
+  Qed.
+
+  Lemma to_list_rows_length_inner st r :
+    List.In r (to_list_rows st) -> length r = Nb.
+  Proof.
+    cbv [to_list_rows]. intro Hin.
+    autorewrite with push_to_list in *.
+    apply List.in_map_iff in Hin.
+    destruct Hin as [? [? ?]]; subst.
+    autorewrite with push_length.
+    reflexivity.
+  Qed.
+
+  Lemma from_big_endian_bytes_to_big_endian_bytes st :
+    from_big_endian_bytes (to_big_endian_bytes st) = st.
+  Proof.
+    cbv [from_big_endian_bytes to_big_endian_bytes].
+    inverse.
+  Qed.
+  Hint Rewrite from_big_endian_bytes_to_big_endian_bytes : inverse.
+
+  Lemma from_cols_to_cols st :
+    from_cols (to_cols st) = st.
+  Proof. cbv [from_cols to_cols]. inverse. Qed.
+  Hint Rewrite from_cols_to_cols : inverse.
+
+  Lemma from_cols_bits_to_cols_bits st :
+    from_cols_bits (to_cols_bits st) = st.
+  Proof. cbv [from_cols_bits to_cols_bits]. inverse. Qed.
+  Hint Rewrite from_cols_bits_to_cols_bits : inverse.
+
+  Lemma from_rows_to_rows st :
+    from_rows (to_rows st) = st.
+  Proof. cbv [from_rows to_rows]. inverse. Qed.
+  Hint Rewrite from_rows_to_rows : inverse.
+
+  Lemma from_list_rows_to_list_rows st :
+    from_list_rows (to_list_rows st) = st.
+  Proof. cbv [from_list_rows to_list_rows]. inverse. Qed.
+  Hint Rewrite from_list_rows_to_list_rows : inverse.
+
+End Properties.
+Hint Rewrite to_big_endian_bytes_from_big_endian_bytes
+     from_big_endian_bytes_to_big_endian_bytes
+     to_cols_from_cols from_cols_to_cols
+     to_cols_bits_from_cols_bits from_cols_bits_to_cols_bits
+     to_rows_from_rows from_rows_to_rows
+     from_list_rows_to_list_rows
+     using solve [eauto] : conversions.
+Hint Rewrite to_list_rows_from_list_rows
+     using solve [length_hammer] : conversions.
+Hint Resolve to_list_rows_length_outer
+     to_list_rows_length_inner : length.
